language_formalisation/type_system/declarational.v
@@ -137,9 +137,6 @@ with has_htype' : ctx -> hcases -> sig -> ctype -> Prop :=
     has_ctype (CtxU (CtxU Γ (TyFun B_op D)) A_op) c_op D ->
     has_htype' 
       Γ (CasesU h op_id x k c_op) (SigU Σ op_id A_op B_op) D
-| TypeHSubtype Γ h Σ Σ' D D' :
-    has_htype Γ h Σ D -> sig_subtype Σ' Σ -> csubtype D D' -> 
-    has_htype' Γ h Σ' D'
 .
 
 
