language_formalisation/type_system/type_aux_lemmas.v
@@ -154,9 +154,6 @@ inv orig. destruct H2.
   - apply IHh; assumption.
   - rewrite ctx_insert_extend. rewrite ctx_insert_extend.
     assert (i+1+1=i+2) by omega. rewrite H5. apply IHc; assumption.
-+ specialize (h_insert_typesafe _ _ _ _ H2) as IHh.
-  clear v_insert_typesafe c_insert_typesafe h_insert_typesafe.
-  eapply TypeHSubtype. apply IHh. all: assumption.
 }
 Qed.
 
@@ -333,9 +330,6 @@ destruct H2.
   - rewrite ctx_remove_extend. rewrite ctx_remove_extend.
     assert (i+1+1=i+2) by omega. rewrite H5.
     apply IHc. destruct no_var. assumption.
-+ specialize (h_negshift_typesafe _ _ _ _ H2) as IHh.
-  clear v_negshift_typesafe c_negshift_typesafe h_negshift_typesafe.
-  eapply TypeHSubtype. apply IHh. all: assumption.
 }
 Qed.
 
@@ -491,27 +485,5 @@ destruct H2.
     rewrite <-(v_shift_shift 1 1 0).
     apply v_shift_typesafe. apply v_shift_typesafe. assumption.
     all: inv H0. 2: assumption. apply WfFun; assumption.
-+ specialize (h_subs_typesafe _ _ _ _ H2) as IHh.
-  clear v_subs_typesafe c_subs_typesafe h_subs_typesafe.
-  eapply TypeHSubtype. eapply IHh. exact gets. all: assumption.
 }
 Qed.
-
-(*
-Lemma h_has_case Γ h Σ D op A_op B_op:
-  has_htype Γ h Σ D ->
-  get_op_type Σ op = Some (A_op, B_op) ->
-  exists x k c_op, find_op_case h op = Some (x, k, c_op).
-Proof.
-revert Γ Σ. induction h; intros Γ Σ typed gets;
-inv typed.
-+ 
-; inv H1; inv H2.
-+ simpl in gets. discriminate.
-+ eapply sig_subtype_gets_Some in gets. 2: exact H6.
-  destruct gets as [A' [B' [gets']]]. rewrite gets in 
-+ simpl in *. destruct (op==o).
-  - injection gets. intros. subst.
-    exists v. exists v0. exists c. reflexivity.
-  - apply IHh in H14; assumption.
-Qed. *)
